SP1Clean/Proofs/Chips/MemoryBumpChip/Formal.lean
@@ -138,8 +138,8 @@ def circuit : GeneralFormalCircuit (ZMod p) Inputs unit where
           | exact Or.inl List.mem_cons_self
           | exact Or.inr List.mem_cons_self
     · intro env h_constraints
-      have h_bool : (ProvableStruct.eval env input_var).is_real = 0 ∨
-          (ProvableStruct.eval env input_var).is_real = 1 := by
+      have h_bool : Expression.eval env input_var.is_real = 0 ∨
+          Expression.eval env input_var.is_real = 1 := by
         apply bool_of_mul_pred
         simpa only [circuit_norm] using h_constraints.1
       rw [Operations.inChannelsOrRequirements_iff_forall_mem]
